examples/pseudo_bool/pbc_normaliseScript.sml
@@ -1210,24 +1210,15 @@ Proof
   simp[satisfiable_normalise,eval_obj_normalise_obj,normalise_thm]
 QED
 
-Definition normalise_output_def:
-  (normalise_output NoOutput = HNoOutput) ∧
-  (normalise_output (Derivable fml) = HDerivable (normalise fml)) ∧
-  (normalise_output (Equisatisfiable fml) = HEquisatisfiable (normalise fml)) ∧
-  (normalise_output (Equioptimal fml obj) =
-    let (obj',fml') = normalise_obj_pbf (obj,fml) in
-      HEquioptimal fml' obj')
-End
-
 Theorem normalise_output_sem_output:
-  normalise_obj_pbf (obj,fml) = (obj',fml') ∧
-  normalise_output output = output' ⇒
-  sem_output (set fml) obj bound output =
-  sem_houtput (set fml') obj' bound output'
+  normalise_obj_pbf (obj1,fml1) = (obj1',fml1') ∧
+  normalise_obj_pbf (obj2,fml2) = (obj2',fml2') ⇒
+  (pbc$sem_output (set fml1) obj1 bound (set fml2) obj2 output ⇔
+  npbc$sem_output (set fml1') obj1' bound (set fml2') obj2' output)
 Proof
   Cases_on`output`>>
-  rw[normalise_output_def,sem_output_def,normalise_obj_pbf_def]>>
-  simp[sem_houtput_def,satisfiable_normalise,eval_obj_normalise_obj,normalise_thm]
+  rw[npbcTheory.sem_output_def,pbcTheory.sem_output_def,normalise_obj_pbf_def]>>
+  simp[satisfiable_normalise,eval_obj_normalise_obj,normalise_thm]
 QED
 
 val _ = export_theory();
